Further progress, isolated step lemma

Layering_Algo.thy
@@ -54,56 +54,6 @@ lemma update_edge_in_E_iff: "e \<in> Graph.E (update_edge c e cap) \<longleftrig
 context Graph
 begin
 
-(*
-definition ebfs_node :: "node \<Rightarrow> _ graph \<Rightarrow> node set \<Rightarrow> (_ graph \<times> node set) nres" where
-  "ebfs_node u c' Q' \<equiv> do {
-    let S = (E``{u}) - (Graph.V c' - Q');
-    c' \<leftarrow> foreach S (\<lambda>v c'. RETURN (update_edge c' (u, v) (c (u, v)))) c';
-    let Q' = Q' \<union> S;
-    RETURN (c', Q')
-  }"
-*)
-
-(* TODO is there a prettier way to phrase "incoming v \<inter> (Graph.V c' \<times> {v})" ? *)
-
-(* TODO this version has an error, as it might add edges from nodes added previously in the same phase *)
-(*
-definition ebfs_node :: "node \<Rightarrow> _ graph \<Rightarrow> node set \<Rightarrow> (_ graph \<times> node set) nres" where
-  "ebfs_node v c' Q' \<equiv> do {
-    c' \<leftarrow> foreach (incoming v \<inter> (Graph.V c' \<times> {v})) (\<lambda>e c'. RETURN (update_edge c' e (c e))) c';
-    let Q' = Q' \<union> (E``{v} - Graph.V c');
-    RETURN (c', Q')
-  }"
-*)
-
-
-
-
-
-
-
-(*
-definition ebfs_node :: "node \<Rightarrow> _ graph \<Rightarrow> node set \<Rightarrow> (_ graph \<times> node set) nres" where
-  "ebfs_node v c' Q' \<equiv> do {
-    c' \<leftarrow> foreach (incoming v \<inter> (Graph.V c' \<times> {v})) (\<lambda>e c'. RETURN (update_edge c' e (c e))) c';
-    let Q' = Q' \<union> (E``{v} - Graph.V c');
-    RETURN (c', Q')
-  }"
-
-definition ebfs_node_invar :: "node \<Rightarrow> _ graph \<Rightarrow> edge set \<Rightarrow> _ graph \<Rightarrow> bool" where
-  "ebfs_node_invar v c_init it c' \<equiv>
-    Subgraph c' c
-    \<and> Graph.E c' \<union> it = Graph.E c_init \<union> (incoming v \<inter> (Graph.V c_init \<times> {v}))"
-
-definition ebfs_phase :: "_ graph \<Rightarrow> node set \<Rightarrow> (_ graph \<times> node set) nres" where
-  "ebfs_phase c' Q \<equiv> foreach Q (\<lambda>u (c', Q'). ebfs_node u c' Q') (c', {})"
-
-definition ebfs_phase_invar :: "node \<Rightarrow> nat \<Rightarrow> node set \<Rightarrow> (_ graph \<times> node set) \<Rightarrow> bool" where
-  "ebfs_phase_invar s n Q \<equiv> \<lambda>(c', Q').
-    S_Shortest_Path_Union c' c s (boundedReachableNodes (Suc n) s - Q)
-    \<and> Q' = exactDistNodes (n + 2) s \<inter> {v. \<exists>u \<in> Graph.V c'. (u, v) \<in> E}"
-*)
-
 subsection \<open>Transferring edges to another graph\<close>
 
 definition transfer_edge :: "edge \<Rightarrow> _ graph \<Rightarrow> _ graph" where
@@ -151,14 +101,6 @@ definition ebfs_phase :: "_ graph \<Rightarrow> node set \<Rightarrow> (_ graph 
       RETURN (c', Q)
     })
     (c\<^sub>i, {})"
-
-(*
-definition ebfs_phase_invar :: "node \<Rightarrow> nat \<Rightarrow> _ graph \<Rightarrow> node set \<Rightarrow> (_ graph \<times> node set) \<Rightarrow> bool" where
-  "ebfs_phase_invar s n c\<^sub>i Q \<equiv> \<lambda>(c', Q').
-    CapacityCompatibleGraphs c' c
-    \<and> Graph.E c' = Graph.E c\<^sub>i \<union> (exactDistNodes n s - Q) \<times> Q'
-    \<and> Q' = exactDistNodes (Suc n) s \<inter> Graph.V c'" (* TODO this part can not be sufficient *)
-*)
 
 definition ebfs_phase_invar :: "node \<Rightarrow> nat \<Rightarrow> _ graph \<Rightarrow> node set \<Rightarrow> (_ graph \<times> node set) \<Rightarrow> bool" where
   "ebfs_phase_invar s n c\<^sub>i Q \<equiv> \<lambda>(c', Q').
@@ -252,38 +194,6 @@ proof
   qed
 qed
 
-
-
-
-
-(*
-  from assms show "S_Shortest_Path_Union c' c s (boundedReachableNodes (Suc n) s)"
-    unfolding ebfs_phase_invar_def by simp
-  then interpret S_Shortest_Path_Union c' c s "boundedReachableNodes (Suc n) s" . (* TODO necessary? *)
-
-  from assms have "Q' = exactDistNodes (n + 2) s \<inter> {v. \<exists>u \<in> Graph.V c'. (u, v) \<in> E}"
-    unfolding ebfs_phase_invar_def by simp
-  moreover have "exactDistNodes (n + 2) s \<subseteq> {v. \<exists>u \<in> Graph.V c'. (u, v) \<in> E}"
-  proof (* TODO prettify *)
-    fix v
-    assume "v \<in> exactDistNodes (n + 2) s"
-    then obtain p where P: "isShortestPath s p v" "length p = n + 2" unfolding exactDistNodes_def
-      by (metis (mono_tags) isShortestPath_min_dist_def mem_Collect_eq obtain_shortest_path)
-    then obtain p\<^sub>u u where "p = p\<^sub>u @ [(u, v)]"
-      by (metis Graph.isPath_bwd_cases add_2_eq_Suc' isShortestPath_def length_Suc_conv list.distinct(1))
-    with P have "isShortestPath s p\<^sub>u u" "length p\<^sub>u = n + 1" "(u, v) \<in> E"
-      using split_shortest_path_around_edge 
-      by (metis Graph.isPath_tail add_Suc_right add_left_imp_eq length_append_singleton nat_1_add_1 plus_1_eq_Suc shortestPath_is_path)+
-    then have "u \<in> boundedReachableNodes (Suc n) s" unfolding boundedReachableNodes_def
-      by (metis connected_def Suc_eq_plus1 isShortestPath_def isShortestPath_min_dist_def mem_Collect_eq)
-    then have "u \<in> V'"
-      by (metis Graph.connected_edgeRtc Graph.connected_inV_iff Graph.distinct_nodes_in_V_if_connected(1) Graph.isPath_rtc Graph.isShortestPath_alt Graph.shortestPath_is_path Graph.simplePath_same_conv Suc_eq_plus1 \<open>isShortestPath s p\<^sub>u u\<close> \<open>length p\<^sub>u = n + 1\<close> insert_iff length_Suc_conv list.distinct(1) shortest_ST_path_remains)
-    with \<open>(u, v) \<in> E\<close> show "v \<in> {v. \<exists>u\<in>V'. (u, v) \<in> E}" by blast
-  qed
-  ultimately show "Q' = exactDistNodes (n + 2) s" by blast
-qed
-*)
-
 context
   (* TODO check where we can be more precise *)
   fixes s
@@ -299,6 +209,39 @@ proof
   then show "finite (Graph.V c')" using FINITE_REACHABLE finite_subset by blast
 qed
 
+lemma ebfs_phase_step:
+  assumes BSPU: "Bounded_S_Shortest_Path_Union c\<^sub>i c s V n"
+    and Q: "u \<in> Q" "Q \<subseteq> exactDistNodes n s"
+    and INVAR: "ebfs_phase_invar s n c\<^sub>i Q (c', Q')"
+  defines "S \<equiv> outgoing u \<inter> {u} \<times> (V - Graph.V c\<^sub>i)"
+  shows "transfer_edges_algo S c' \<le> (spec c''. ebfs_phase_invar s n c\<^sub>i (Q - {u}) (c'', Q' \<union> snd ` S))"
+proof -
+  from Q have "connected s u" unfolding exactDistNodes_def by blast
+  then have "outgoing u \<subseteq> {u} \<times> reachableNodes s"
+    unfolding outgoing_def reachableNodes_def using connected_append_edge by blast
+  with FINITE_REACHABLE have "finite S" unfolding S_def using finite_subset by blast
+  then have "transfer_edges_algo S c' \<le> return (transfer_edges S c')"
+    using transfer_edges_correct by blast
+  also have "... \<le> (spec c''. ebfs_phase_invar s n c\<^sub>i (Q - {u}) (c'', Q' \<union> snd ` S))"
+    unfolding ebfs_phase_invar_def
+  proof (clarify, refine_vcg)
+    from INVAR have "CapacityCompatibleGraphs c' c"
+      and E'_EQ: "Graph.E c' = Graph.E c\<^sub>i \<union> E \<inter> (exactDistNodes n s - Q) \<times> Q'"
+      and Q'_EQ: "Q' = exactDistNodes (Suc n) s \<inter> E `` (exactDistNodes n s - Q)"
+      unfolding ebfs_phase_invar_def by auto
+    then interpret CapacityCompatibleGraphs c' c by simp
+    from BSPU interpret g\<^sub>i: Bounded_S_Shortest_Path_Union c\<^sub>i c s V n .
+
+    show "CapacityCompatibleGraphs (transfer_edges S c') c"
+      using \<open>CapacityCompatibleGraphs c' c\<close> transfer_edges_capcomp by blast
+
+    show "Q' \<union> snd ` S = exactDistNodes (Suc n) s \<inter> E `` (exactDistNodes n s - (Q - {u}))" sorry
+
+    show "Graph.E (transfer_edges S c') = g\<^sub>i.E' \<union> E \<inter> (exactDistNodes n s - (Q - {u})) \<times> (Q' \<union> snd ` S)" sorry
+  qed
+  finally show ?thesis .
+qed
+
 lemma ebfs_phase_correct:
   fixes c' Q n
   assumes BSPU: "Bounded_S_Shortest_Path_Union c' c s V n"
@@ -306,9 +249,7 @@ lemma ebfs_phase_correct:
   unfolding ebfs_phase_def
   apply (refine_vcg FOREACH_rule[where I="ebfs_phase_invar s n c'"])
   using FINITE_REACHABLE finite_subset exactDistNodes_reachable_ss boundedReachableNodes_ss apply meson
-  using BSPU ebfs_phase_initial apply simp
-
-  using ebfs_phase_final[OF BSPU] apply simp_all
+  using BSPU ebfs_phase_initial ebfs_phase_step ebfs_phase_final by simp_all
 end
 
 
@@ -318,226 +259,6 @@ end
 
 
 
-
-
-
-(*
-lemma ebfs_phase_correct:
-  fixes s c' Q n
-  assumes FIN: "finite (reachableNodes s)" (*"finite (exactDistNodes n s)"*)
-    and SPU: "S_Shortest_Path_Union c' c s (boundedReachableNodes n s)"
-  shows "ebfs_phase c' (exactDistNodes n s) \<le> SPEC (\<lambda>(c'', Q'). S_Shortest_Path_Union c'' c s (boundedReachableNodes (Suc n) s) \<and> Q' = exactDistNodes (Suc n) s)"
-  unfolding ebfs_phase_def
-  apply (refine_vcg FOREACH_rule[where I="ebfs_phase_invar s n c'"])
-  using FIN finite_subset exactDistNodes_reachable_ss boundedReachableNodes_ss apply meson
-  using ebfs_phase_initial[OF SPU] apply simp
-  using assms ebfs_phase_initial ebfs_phase_step ebfs_phase_final by simp_all
-*)
-
-
-
-
-
-
-
-
-
-
-
-
-
-
-
-
-
-
-
-
-
-lemma ebfs_node_final:
-  assumes V_DIST: "v \<in> Q" "Q \<subseteq> exactDistNodes (Suc n) s" (* TODO what exactly do we need here? *)
-    and NODE_INVAR: "ebfs_node_invar v c_init {} c'"
-    and PHASE_INVAR: "ebfs_phase_invar s n Q (c_init, Q')"
-  shows "ebfs_phase_invar s n (Q - {v}) (c', Q' \<union> (E `` {v} - Graph.V c'))"
-  unfolding ebfs_phase_invar_def
-proof (intro case_prodI conjI)
-  from NODE_INVAR interpret Subgraph c' c unfolding ebfs_node_invar_def by blast
-
-  from PHASE_INVAR interpret init: S_Shortest_Path_Union c_init c s "boundedReachableNodes (Suc n) s - Q"
-    unfolding ebfs_phase_invar_def by blast
-
-  thm assms[unfolded ebfs_node_invar_def ebfs_phase_invar_def, simplified]
-  show "S_Shortest_Path_Union c' c s (boundedReachableNodes (Suc n) s - (Q - {v}))"
-  proof (unfold_locales, intro equalityI; intro subsetI)
-    fix e
-    assume "e \<in> E'"
-    then consider (old_edge) "e \<in> Graph.E c_init"
-      | (new_edge) "e \<in> incoming v \<inter> Graph.V c_init \<times> {v}"
-      using NODE_INVAR unfolding ebfs_node_invar_def by blast
-    then show "e \<in> \<Union> {set p |p. \<exists>t. t \<in> boundedReachableNodes (Suc n) s - (Q - {v}) \<and> isShortestPath s p t}"
-    proof cases
-      case old_edge
-      then obtain t p where "t \<in> boundedReachableNodes (Suc n) s - Q" "isShortestPath s p t" "e \<in> set p"
-        using init.shortest_s_path_union by fast
-      then show ?thesis by blast
-    next
-      case new_edge
-      then obtain u where "u \<in> Graph.V c_init" "(u, v) \<in> E" and [simp]: "e = (u, v)"
-        unfolding incoming_def Graph.V_def Graph.E_def by blast
-      (*then obtain p where "isShortestPath s p u" "length p \<le> n" oops*)
-      then show ?thesis sorry
-    qed
-  next
-    fix e
-    assume "e \<in> \<Union> {set p |p. \<exists>t. t \<in> boundedReachableNodes (Suc n) s - (Q - {v}) \<and> isShortestPath s p t}"
-    then consider p t where "e \<in> set p" "t \<in> boundedReachableNodes (Suc n) s - Q" "isShortestPath s p t"
-      | p where "e \<in> set p" "isShortestPath s p v" by blast
-    then show "e \<in> E'"
-    proof cases
-      case 1
-      then show ?thesis sorry
-    next
-      case 2
-      then show ?thesis sorry
-    qed
-  qed
-
-  (* TODO *)
-  have "init.V' = V' - {v}" using NODE_INVAR unfolding ebfs_node_invar_def Graph.V_def sorry
-  have "{v. \<exists>u\<in>init.V'. (u, v) \<in> E} \<union> (E `` {v}) = {v. \<exists>u\<in>V'. (u, v) \<in> E}"
-
-  thm assms[unfolded ebfs_node_invar_def ebfs_phase_invar_def, simplified]
-  have "Q' \<union> (E `` {v} - V') = exactDistNodes (n + 2) s \<inter> {v. \<exists>u\<in>init.V'. (u, v) \<in> E} \<union> (E `` {v} - V')"
-    using PHASE_INVAR unfolding ebfs_phase_invar_def by fast
-  also have "... = exactDistNodes (n + 2) s \<inter> {v. \<exists>u\<in>init.V'. (u, v) \<in> E} \<union> (E `` {v} - V')" sorry
-
-  show "Q' \<union> (E `` {v} - V') = exactDistNodes (n + 2) s \<inter> {v. \<exists>u\<in>V'. (u, v) \<in> E}"
-    using assms[unfolded ebfs_node_invar_def ebfs_phase_invar_def, simplified] oops
-qed
-
-lemma ebfs_phase_initial:
-  assumes "S_Shortest_Path_Union c' c s (boundedReachableNodes n s)"
-  shows "ebfs_phase_invar s n (exactDistNodes (Suc n) s) (c', {})"
-  unfolding ebfs_phase_invar_def
-proof (intro case_prodI conjI)
-  show "S_Shortest_Path_Union c' c s (boundedReachableNodes (Suc n) s - exactDistNodes (Suc n) s)"
-    using assms by (simp add: ebfs_phase_invar_def exactDistNodes_alt boundedReachableNodes_mono double_diff)
-
-  have "\<And>v. \<exists>u \<in> Graph.V c'. (u, v) \<in> E \<Longrightarrow> v \<notin> exactDistNodes (n + 2) s"
-  proof -
-    interpret S_Shortest_Path_Union c' c s "boundedReachableNodes n s" using assms .
-
-    fix v
-    assume "\<exists>u \<in> Graph.V c'. (u, v) \<in> E"
-    then obtain u where "u \<in> Graph.V c'" "(u, v) \<in> E" by blast
-    then obtain t p\<^sub>s p\<^sub>t where "t \<in> boundedReachableNodes n s" "isShortestPath s (p\<^sub>s @ p\<^sub>t) t"
-      and P2: "isShortestPath s p\<^sub>s u"
-      by (blast elim: obtain_shortest_ST_paths)
-    then have "length p\<^sub>s \<le> n" unfolding boundedReachableNodes_def isShortestPath_min_dist_def by simp
-    with P2 \<open>(u, v) \<in> E\<close> have "min_dist s v \<le> Suc n"
-      using isShortestPath_min_dist_def connected_def min_dist_succ by fastforce
-    then show "v \<notin> exactDistNodes (n + 2) s" unfolding exactDistNodes_def by simp
-  qed
-  then show "{} = exactDistNodes (n + 2) s \<inter> {v. \<exists>u\<in>Graph.V c'. (u, v) \<in> E}" by blast
-qed
-
-lemma ebfs_phase_final:
-  assumes "ebfs_phase_invar s n {} (c', Q')"
-  shows "S_Shortest_Path_Union c' c s (boundedReachableNodes (Suc n) s) \<and> Q' = exactDistNodes (n + 2) s"
-proof
-  from assms show "S_Shortest_Path_Union c' c s (boundedReachableNodes (Suc n) s)"
-    unfolding ebfs_phase_invar_def by simp
-  then interpret S_Shortest_Path_Union c' c s "boundedReachableNodes (Suc n) s" . (* TODO necessary? *)
-
-  from assms have "Q' = exactDistNodes (n + 2) s \<inter> {v. \<exists>u \<in> Graph.V c'. (u, v) \<in> E}"
-    unfolding ebfs_phase_invar_def by simp
-  moreover have "exactDistNodes (n + 2) s \<subseteq> {v. \<exists>u \<in> Graph.V c'. (u, v) \<in> E}"
-  proof (* TODO prettify *)
-    fix v
-    assume "v \<in> exactDistNodes (n + 2) s"
-    then obtain p where P: "isShortestPath s p v" "length p = n + 2" unfolding exactDistNodes_def
-      by (metis (mono_tags) isShortestPath_min_dist_def mem_Collect_eq obtain_shortest_path)
-    then obtain p\<^sub>u u where "p = p\<^sub>u @ [(u, v)]"
-      by (metis Graph.isPath_bwd_cases add_2_eq_Suc' isShortestPath_def length_Suc_conv list.distinct(1))
-    with P have "isShortestPath s p\<^sub>u u" "length p\<^sub>u = n + 1" "(u, v) \<in> E"
-      using split_shortest_path_around_edge 
-      by (metis Graph.isPath_tail add_Suc_right add_left_imp_eq length_append_singleton nat_1_add_1 plus_1_eq_Suc shortestPath_is_path)+
-    then have "u \<in> boundedReachableNodes (Suc n) s" unfolding boundedReachableNodes_def
-      by (metis connected_def Suc_eq_plus1 isShortestPath_def isShortestPath_min_dist_def mem_Collect_eq)
-    then have "u \<in> V'"
-      by (metis Graph.connected_edgeRtc Graph.connected_inV_iff Graph.distinct_nodes_in_V_if_connected(1) Graph.isPath_rtc Graph.isShortestPath_alt Graph.shortestPath_is_path Graph.simplePath_same_conv Suc_eq_plus1 \<open>isShortestPath s p\<^sub>u u\<close> \<open>length p\<^sub>u = n + 1\<close> insert_iff length_Suc_conv list.distinct(1) shortest_ST_path_remains)
-    with \<open>(u, v) \<in> E\<close> show "v \<in> {v. \<exists>u\<in>V'. (u, v) \<in> E}" by blast
-  qed
-  ultimately show "Q' = exactDistNodes (n + 2) s" by blast
-qed
-
-context
-  (* TODO check where we can be more precise *)
-  fixes s
-  assumes FINITE_REACHABLE: "finite (reachableNodes s)"
-begin
-lemma finite_if_spu[intro]: "S_Shortest_Path_Union c' c s T \<Longrightarrow> Finite_Graph c'"
-proof
-  assume "S_Shortest_Path_Union c' c s T"
-  then interpret S_Shortest_Path_Union c' c s T .
-  have "Graph.V c' \<subseteq> reachableNodes s"
-    unfolding reachableNodes_def using sg_connected_remains_base_connected by blast
-  then show "finite (Graph.V c')" using FINITE_REACHABLE finite_subset by blast
-qed
-
-lemma ebfs_node_step:
-  assumes "e \<in> it" "it \<subseteq> incoming v \<inter> V' \<times> {v}" and INVAR: "ebfs_node_invar v c_init it c'"
-  shows "ebfs_node_invar v c_init (it - {e}) (update_edge c' e (c e))"
-proof -
-  from assms have "c e \<noteq> 0"
-    using Graph.incoming_edges Graph.E_def unfolding split_paired_all by blast
-  with \<open>e \<in> it\<close> INVAR show ?thesis unfolding ebfs_node_invar_def by auto
-qed
-
-lemma ebfs_phase_step:
-  assumes "u \<in> Q" and "Q \<subseteq> exactDistNodes (Suc n) s" and INVAR: "ebfs_phase_invar s n Q (c', Q')"
-  shows "ebfs_node u c' Q' \<le> SPEC (ebfs_phase_invar s n (Q - {u}))"
-proof -
-  from INVAR interpret S_Shortest_Path_Union c' c s "boundedReachableNodes (Suc n) s - Q"
-    unfolding ebfs_phase_invar_def by blast
-
-  show ?thesis
-  unfolding ebfs_node_def
-  apply (refine_vcg FOREACH_rule[where I="ebfs_node_invar u c'"])
-  using S_Shortest_Path_Union_axioms apply (blast intro: Finite_Graph.finite_V)
-  using Subgraph_axioms apply (simp add: ebfs_node_invar_def) (* TODO can this work without the interpretation setup? *)
-  using ebfs_node_step oops apply blast
-  using ebfs_node_final assms by fast
-qed
-end
-
-(*
-lemma ebfs_phase_correct:
-  fixes s c' Q n
-  assumes "finite (reachableNodes s)" (*"finite (exactDistNodes (Suc n) s)"*)
-    and "S_Shortest_Path_Union c' c s (boundedReachableNodes n s)"
-  shows "ebfs_phase c' (exactDistNodes (Suc n) s) \<le> SPEC(\<lambda>(c'', Q'). S_Shortest_Path_Union c'' c s (boundedReachableNodes (Suc n) s) \<and> Q' = exactDistNodes (n + 2) s)"
-  unfolding ebfs_phase_def
-  apply (refine_vcg FOREACH_rule[where I="ebfs_phase_invar s n"])
-  using assms finite_subset sorry  apply (metis Diff_subset exactDistNodes_alt boundedReachableNodes_ss)
-  using assms ebfs_phase_initial ebfs_phase_step ebfs_phase_final by simp_all
-*)
-
-thm FOREACH_rule
-(* TODO somewhere we need the fact that the set of reachable nodes (from s) is finite *)
-
-(* TODO is it better to remove any notion of Bounded locales from this part and rely entirely on restricted reachable sets? *)
-(*
-lemma ebfs_phase_correct:
-  fixes s c' Q n
-  assumes "Bounded_S_Shortest_Path_Union c' c s V n"
-    and "Q = {u. connected s u \<and> min_dist s u = n + 1}"
-    and "finite Q"
-  shows "ebfs_phase c' Q \<le> SPEC(\<lambda>(c'', Q'). Bounded_S_Shortest_Path_Union c'' c s V (n + 1) \<and> Q' = {u. connected s u \<and> min_dist s u = n + 2})"
-  unfolding ebfs_phase_def
-  apply (rule FOREACH_rule, clarsimp_all)
-proof (refine_vcg)
-*)
 
 
 
